pcuic/theories/PCUICCumulativity.v
@@ -1,4 +1,6 @@
 (* Distributed under the terms of the MIT license. *)
+From Coq Require Import CRelationClasses.
+From Equations.Type Require Import Relation Relation_Properties.
 From MetaCoq.Template Require Import config utils BasicAst.
 From MetaCoq.PCUIC Require Import PCUICAst PCUICAstUtils
      PCUICLiftSubst PCUICEquality PCUICUnivSubst PCUICReduction.
